Updates.

FOL/NV/Sub/Pred/One/Ind/Sub.lean
@@ -11,9 +11,9 @@ open Formula_
 /--
   The inductive simultaneous uniform substitution of a single predicate variable in a formula.
 
-  IsSub A P zs H B := The formula A is said to be transformed into the formula B by a substitution of H* for P z₁ ... zₙ, abbreviated: Sub A (P zⁿ / H*) B, iff B is obtained from A upon replacing in A each occurrence of a derivative of the name form P z₁ ... zₙ by the corresponding derivative of the substituend H*, provided that: (i) P does not occur in a component formula (∀ x A₁) of A if x is a parameter of H*, and (ii) the name variable zₖ, k = 1, ..., n, is not free in a component formula (∀ x H) of H* if P t₁ ... tₙ occurs in A with x occurring in tₖ. If conditions (i) and (ii) are not satisfied, then the indicated substitution for predicate variables is left undefined.
+  is_sub_pred_one_ind A P zs H B := The formula A is said to be transformed into the formula B by a substitution of H* for P z₁ ... zₙ, abbreviated: Sub A (P zⁿ / H*) B, iff B is obtained from A upon replacing in A each occurrence of a derivative of the name form P z₁ ... zₙ by the corresponding derivative of the substituend H*, provided that: (i) P does not occur in a component formula (∀ x A₁) of A if x is a parameter of H*, and (ii) the name variable zₖ, k = 1, ..., n, is not free in a component formula (∀ x H) of H* if P t₁ ... tₙ occurs in A with x occurring in tₖ. If conditions (i) and (ii) are not satisfied, then the indicated substitution for predicate variables is left undefined.
 -/
-inductive IsSub
+inductive is_sub_pred_one_ind
   (P : PredName_)
   (zs : List VarName_)
   (H : Formula_) :
@@ -22,7 +22,7 @@ inductive IsSub
   | pred_const_
     (X : PredName_)
     (xs : List VarName_) :
-    IsSub P zs H (pred_const_ X xs) (pred_const_ X xs)
+    is_sub_pred_one_ind P zs H (pred_const_ X xs) (pred_const_ X xs)
 
 /-
   If A is an atomic formula not containing P then Sub A (P zⁿ / H*) A.
@@ -32,7 +32,7 @@ inductive IsSub
     (X : PredName_)
     (xs : List VarName_) :
     ¬ (X = P ∧ xs.length = zs.length) →
-    IsSub P zs H (pred_var_ X xs) (pred_var_ X xs)
+    is_sub_pred_one_ind P zs H (pred_var_ X xs) (pred_var_ X xs)
 
   /-
   If A = P t₁ ... tₙ and Sf H* (zⁿ / tⁿ) B, then Sub A (P zⁿ / H*) B.
@@ -47,16 +47,16 @@ inductive IsSub
     (ts : List VarName_) :
     X = P ∧ ts.length = zs.length →
     Sub.Var.All.Rec.admits_var_all_rec (Function.updateListITE id zs ts) H →
-    IsSub P zs H (pred_var_ P ts)
+    is_sub_pred_one_ind P zs H (pred_var_ P ts)
     (Sub.Var.All.Rec.fast_replace_free_var_all_rec (Function.updateListITE id zs ts) H)
 
   | eq_
     (x y : VarName_) :
-    IsSub P zs H (eq_ x y) (eq_ x y)
+    is_sub_pred_one_ind P zs H (eq_ x y) (eq_ x y)
 
-  | true_ : IsSub P zs H true_ true_
+  | true_ : is_sub_pred_one_ind P zs H true_ true_
 
-  | false_ : IsSub P zs H false_ false_
+  | false_ : is_sub_pred_one_ind P zs H false_ false_
 
 /-
   If A = (¬ A₁) and Sub A₁ (P zⁿ / H*) B₁, then Sub A (P zⁿ / H*) (¬ B₁).
@@ -64,8 +64,8 @@ inductive IsSub
   | not_
     (phi : Formula_)
     (phi' : Formula_) :
-    IsSub P zs H phi phi' →
-    IsSub P zs H phi.not_ phi'.not_
+    is_sub_pred_one_ind P zs H phi phi' →
+    is_sub_pred_one_ind P zs H phi.not_ phi'.not_
 
 /-
   If A = (A₁ → A₂), Sub A₁ (P zⁿ / H*) B₁, and Sub A₂ (P zⁿ / H*) B₂, then Sub A (P zⁿ / H*) (B₁ → B₁).
@@ -74,30 +74,30 @@ inductive IsSub
   | imp_
     (phi psi : Formula_)
     (phi' psi' : Formula_) :
-    IsSub P zs H phi phi' →
-    IsSub P zs H psi psi' →
-    IsSub P zs H (phi.imp_ psi) (phi'.imp_ psi')
+    is_sub_pred_one_ind P zs H phi phi' →
+    is_sub_pred_one_ind P zs H psi psi' →
+    is_sub_pred_one_ind P zs H (phi.imp_ psi) (phi'.imp_ psi')
 
   | and_
     (phi psi : Formula_)
     (phi' psi' : Formula_) :
-    IsSub P zs H phi phi' →
-    IsSub P zs H psi psi' →
-    IsSub P zs H (phi.and_ psi) (phi'.and_ psi')
+    is_sub_pred_one_ind P zs H phi phi' →
+    is_sub_pred_one_ind P zs H psi psi' →
+    is_sub_pred_one_ind P zs H (phi.and_ psi) (phi'.and_ psi')
 
   | or_
     (phi psi : Formula_)
     (phi' psi' : Formula_) :
-    IsSub P zs H phi phi' →
-    IsSub P zs H psi psi' →
-    IsSub P zs H (phi.or_ psi) (phi'.or_ psi')
+    is_sub_pred_one_ind P zs H phi phi' →
+    is_sub_pred_one_ind P zs H psi psi' →
+    is_sub_pred_one_ind P zs H (phi.or_ psi) (phi'.or_ psi')
 
   | iff_
     (phi psi : Formula_)
     (phi' psi' : Formula_) :
-    IsSub P zs H phi phi' →
-    IsSub P zs H psi psi' →
-    IsSub P zs H (phi.iff_ psi) (phi'.iff_ psi')
+    is_sub_pred_one_ind P zs H phi phi' →
+    is_sub_pred_one_ind P zs H psi psi' →
+    is_sub_pred_one_ind P zs H (phi.iff_ psi) (phi'.iff_ psi')
 
 
 /-
@@ -111,21 +111,21 @@ inductive IsSub
     (phi : Formula_)
     (phi' : Formula_) :
     ¬ var_is_free_in x H →
-    IsSub P zs H phi phi' →
-    IsSub P zs H (forall_ x phi) (forall_ x phi')
+    is_sub_pred_one_ind P zs H phi phi' →
+    is_sub_pred_one_ind P zs H (forall_ x phi) (forall_ x phi')
 
   | exists_
     (x : VarName_)
     (phi : Formula_)
     (phi' : Formula_) :
     ¬ var_is_free_in x H →
-    IsSub P zs H phi phi' →
-    IsSub P zs H (exists_ x phi) (exists_ x phi')
+    is_sub_pred_one_ind P zs H phi phi' →
+    is_sub_pred_one_ind P zs H (exists_ x phi) (exists_ x phi')
 
   | def_
     (X : DefName_)
     (xs : List VarName_) :
-    IsSub P zs H (def_ X xs) (def_ X xs)
+    is_sub_pred_one_ind P zs H (def_ X xs) (def_ X xs)
 
 
 theorem substitution_theorem
@@ -138,7 +138,7 @@ theorem substitution_theorem
   (zs : List VarName_)
   (H : Formula_)
   (B : Formula_)
-  (h1 : IsSub P zs H A B)
+  (h1 : is_sub_pred_one_ind P zs H A B)
   (h2 : ∀ (Q : PredName_) (ds : List D),
     Q = P ∧ ds.length = zs.length →
       (holds D I (Function.updateListITE V zs ds) E H ↔ J.pred_var_ P ds))
@@ -250,7 +250,7 @@ theorem substitution_is_valid
   (P : PredName_)
   (zs : List VarName_)
   (H : Formula_)
-  (h1 : IsSub P zs H F F')
+  (h1 : is_sub_pred_one_ind P zs H F F')
   (h2 : F.is_valid) :
   F'.is_valid :=
   by
